@prefix rdf: <http://www.w3.org/1999/02/22-rdf-syntax-ns#> .
@prefix dc: <http://purl.org/dc/elements/1.1/> .
@prefix skos: <http://www.w3.org/2004/02/skos/core#> .
@prefix foo: <http://www.foo.org/foo/> .

<http://opencoredata.org/voc/janus/1/>
    dc:creator "Open Core Data" ;
    dc:description "A vocabulary for describing parameters used in the DSDP/OPD/IODP Janus Database" ;
    dc:title "OCD Janus Controlled Vocabulary" ;
    a skos:ConceptScheme .

<http://opencoredata.org/voc/janus/1/janusagemodel>
    a skos:Concept ;
    skos:definition "Age model (or Age Depth Model) interpretations based mostly on paleontological but also paleomagnetic and radio-isotopic analyses." ;
    skos:inScheme <http://opencoredata.org/voc/janus/1/> .

<http://opencoredata.org/voc/janus/1/janusageprofile>
    a skos:Concept ;
    skos:definition "Interpretations of fossil datums used to construct age models for holes." ;
    skos:inScheme <http://opencoredata.org/voc/janus/1/> .

<http://opencoredata.org/voc/janus/1/januschemcarb>
    a skos:Concept ;
    skos:definition "Measurements of carbonate data generated from instrumentation in the shipboard chemistry lab including weight percentages of inorganic, organic, and total carbon, calcium carbonate, nitrogen, sulfur, and hydrogen." ;
    skos:inScheme <http://opencoredata.org/voc/janus/1/> .

<http://opencoredata.org/voc/janus/1/januschemcarbtest>
    a skos:Concept ;
    skos:definition "Test for retrieving additional depth types (mcd) and depth options  (voids, exotics, compression), and formatted strings for float measurement fields for writing to datasets." ;
    skos:inScheme <http://opencoredata.org/voc/janus/1/> .

<http://opencoredata.org/voc/janus/1/januschemgas>
    a skos:Concept ;
    skos:definition "NEW:  Measurements of gas elements generated using gas chromatographs and natural gas analyzers in the shipboad chemistry lab." ;
    skos:inScheme <http://opencoredata.org/voc/janus/1/> .

<http://opencoredata.org/voc/janus/1/januschemiw>
    a skos:Concept ;
    skos:definition "NEW:  Measurements of elements,  compounds, salinity, alkalinity, and pH from interstitial (pore) water samples generated using gas chromatography, mass spectrometry, and atomic emissions spectrometry in the shipboard chemistry lab." ;
    skos:inScheme <http://opencoredata.org/voc/janus/1/> .

<http://opencoredata.org/voc/janus/1/januschemrockeval>
    a skos:Concept ;
    skos:definition "NEW:  Measurements of type and maturity of organic carbon and hydrocarbon potential (for safety purposes) by sample pyrolysis using RockEval instrumentation." ;
    skos:inScheme <http://opencoredata.org/voc/janus/1/> .

<http://opencoredata.org/voc/janus/1/januscorecloseupimage>
    a skos:Concept ;
    skos:definition "NEW:  URL links to closeup core photo images." ;
    skos:inScheme <http://opencoredata.org/voc/janus/1/> .

<http://opencoredata.org/voc/janus/1/januscoreimage>
    a skos:Concept ;
    skos:definition "URL links to core and core-section photo images." ;
    skos:inScheme <http://opencoredata.org/voc/janus/1/> .

<http://opencoredata.org/voc/janus/1/januscorelogsummary>
    a skos:Concept ;
    skos:definition "NOT NEEDED, SEE OCD_CORE_SECTION_SUMMARY" ;
    skos:inScheme <http://opencoredata.org/voc/janus/1/> .

<http://opencoredata.org/voc/janus/1/januscoresample>
    a skos:Concept ;
    skos:definition "Information on samples taken from cores for shipboard laboratories to fulfill minimum data requirements and post-cruise for research proposals." ;
    skos:inScheme <http://opencoredata.org/voc/janus/1/> .

<http://opencoredata.org/voc/janus/1/januscoresampletotal>
    a skos:Concept ;
    skos:definition "NEW:  Summary statistics regarding the number of samples taken for particular laboratory purposes or in fulfillment of a sample request." ;
    skos:inScheme <http://opencoredata.org/voc/janus/1/> .

<http://opencoredata.org/voc/janus/1/januscoresectionsummary>
    a skos:Concept ;
    skos:definition "NEW:  Summary of core and section depths and offsets." ;
    skos:inScheme <http://opencoredata.org/voc/janus/1/> .

<http://opencoredata.org/voc/janus/1/januscoresummary>
    a skos:Concept ;
    skos:definition "Summary of core depth intervals and offsets." ;
    skos:inScheme <http://opencoredata.org/voc/janus/1/> .

<http://opencoredata.org/voc/janus/1/januscryomag>
    a skos:Concept ;
    skos:definition "Measurements of paleomagnetic data including declination, inclination and intensity taken with a cryogenic magnetometer and other equipment." ;
    skos:inScheme <http://opencoredata.org/voc/janus/1/> .

<http://opencoredata.org/voc/janus/1/janusdht>
    a skos:Concept ;
    skos:definition "Measurements of downhole temperature." ;
    skos:inScheme <http://opencoredata.org/voc/janus/1/> .

<http://opencoredata.org/voc/janus/1/janusdigitalrgb>
    a skos:Concept ;
    skos:definition "NEW:  Measurements of red, green, blue (RGB) values taken on cores with a line-scan camera." ;
    skos:inScheme <http://opencoredata.org/voc/janus/1/> .

<http://opencoredata.org/voc/janus/1/janusgra>
    a skos:Concept ;
    skos:definition "Measurements of gamma-ray attenuation and calculated bulk density acquired using sensors on the whole-core multi-sensing track (WC-MST)." ;
    skos:inScheme <http://opencoredata.org/voc/janus/1/> .

<http://opencoredata.org/voc/janus/1/janusicpaes>
    a skos:Concept ;
    skos:definition "Measurements of major and trace elements by geochemical analyses using inductively coupled plasma-atomic emmission spectrometry (ICP-AES)." ;
    skos:inScheme <http://opencoredata.org/voc/janus/1/> .

<http://opencoredata.org/voc/janus/1/januslimscomponentref>
    a skos:Concept ;
    skos:definition "NEW:  Reference for LIMS Components" ;
    skos:inScheme <http://opencoredata.org/voc/janus/1/> .

<http://opencoredata.org/voc/janus/1/janusmad>
    a skos:Concept ;
    skos:definition "Index Properties of Moisture and Density (MAD) including moisture content, porosity, and void ratio derived from measurements from pycnometers and mass balances." ;
    skos:inScheme <http://opencoredata.org/voc/janus/1/> .

<http://opencoredata.org/voc/janus/1/janusmiscmetadata>
    a skos:Concept ;
    skos:definition "NEW:  Miscellaneous metadata on instrumentation, analyses, and measurements." ;
    skos:inScheme <http://opencoredata.org/voc/janus/1/> .

<http://opencoredata.org/voc/janus/1/janusmiscspecialhole>
    a skos:Concept ;
    skos:definition "NEW:  Location and coring information on designated special holes." ;
    skos:inScheme <http://opencoredata.org/voc/janus/1/> .

<http://opencoredata.org/voc/janus/1/janusms2f>
    a skos:Concept ;
    skos:definition "Measurements of point magnetic susceptibility acquired using a meter attached to the Archive Half Multisensor Track (AMST) in the shipboard environment." ;
    skos:inScheme <http://opencoredata.org/voc/janus/1/> .

<http://opencoredata.org/voc/janus/1/janusmscl>
    a skos:Concept ;
    skos:definition "Measurements of magnetic susceptibility acquired using a core logger configurable with one or two Bartington magnetic susceptibility sensors affixed to a push-rod style GeoTek rail system (MSCL)." ;
    skos:inScheme <http://opencoredata.org/voc/janus/1/> .

<http://opencoredata.org/voc/janus/1/janusmsl>
    a skos:Concept ;
    skos:definition "Measurements of magnetic susceptibility acquired using a Bartington loop affixed to the whole-core multi-sensor track (WC-MST)." ;
    skos:inScheme <http://opencoredata.org/voc/janus/1/> .

<http://opencoredata.org/voc/janus/1/janusncr>
    a skos:Concept ;
    skos:definition "Measurements of non-contact resistivity (NCR) derived from GeoTek instrumentation." ;
    skos:inScheme <http://opencoredata.org/voc/janus/1/> .

<http://opencoredata.org/voc/janus/1/janusngr>
    a skos:Concept ;
    skos:definition "Measurements of natural gamma radiation (NGR) counts acquired using NaI sensors on the whole-core multi-sensor track (WC-MST) system." ;
    skos:inScheme <http://opencoredata.org/voc/janus/1/> .

<http://opencoredata.org/voc/janus/1/januspaleodatumref>
    a skos:Concept ;
    skos:definition "NEW:  Reference listing of taxon datum concepts." ;
    skos:inScheme <http://opencoredata.org/voc/janus/1/> .

<http://opencoredata.org/voc/janus/1/januspaleoimage>
    a skos:Concept ;
    skos:definition "Url links to prime data images of scanned Paleontology and Biostratigraphy log sheets. " ;
    skos:inScheme <http://opencoredata.org/voc/janus/1/> .

<http://opencoredata.org/voc/janus/1/januspaleooccurrence>
    a skos:Concept ;
    skos:definition "Fossil taxa occurrence (abundance and preservation) data, and age/zonation identification on a species by species basis for each sample." ;
    skos:inScheme <http://opencoredata.org/voc/janus/1/> .

<http://opencoredata.org/voc/janus/1/januspaleorangetable>
    a skos:Concept ;
    skos:definition "DELETE:  SEE OCD_PALEO_OCCURRENCE" ;
    skos:inScheme <http://opencoredata.org/voc/janus/1/> .

<http://opencoredata.org/voc/janus/1/januspaleosampleinterp>
    a skos:Concept ;
    skos:definition "Interpretations at a sample-level by fossil group of abundance, preservation, geological age range, zonation range, paleobathymetry, and comments." ;
    skos:inScheme <http://opencoredata.org/voc/janus/1/> .

<http://opencoredata.org/voc/janus/1/januspaleotaxonomyref>
    a skos:Concept ;
    skos:definition "NEW:  Reference listing of taxon species concepts." ;
    skos:inScheme <http://opencoredata.org/voc/janus/1/> .

<http://opencoredata.org/voc/janus/1/januspaleozoneref>
    a skos:Concept ;
    skos:definition "NEW:  Reference listing of taxon zone concepts." ;
    skos:inScheme <http://opencoredata.org/voc/janus/1/> .

<http://opencoredata.org/voc/janus/1/janusprimedataimage>
    a skos:Concept ;
    skos:definition "URL links to scanned images of prime data types including visual core description (VCD), Paleontology, VCD hard rock, VCD structual, and X-ray diffraction (XRD)." ;
    skos:inScheme <http://opencoredata.org/voc/janus/1/> .

<http://opencoredata.org/voc/janus/1/januspwl>
    a skos:Concept ;
    skos:definition "Measurements of P-wave velocity collected by the sonic velocity sensor on a whole-core multi-sensing track (WC-MST) system." ;
    skos:inScheme <http://opencoredata.org/voc/janus/1/> .

<http://opencoredata.org/voc/janus/1/januspws1>
    a skos:Concept ;
    skos:definition "Measurements of P-wave velocity in the z-direction on split cores." ;
    skos:inScheme <http://opencoredata.org/voc/janus/1/> .

<http://opencoredata.org/voc/janus/1/januspws2>
    a skos:Concept ;
    skos:definition "Measurements of P-wave velocity in the y-direction on split cores." ;
    skos:inScheme <http://opencoredata.org/voc/janus/1/> .

<http://opencoredata.org/voc/janus/1/januspws3>
    a skos:Concept ;
    skos:definition "Measurements of P-wave velocity in the x-direction on split cores with or without core liners, and in the x, y, and z-directions on cubic or cylindrical, consolidated, or lithified core specimens." ;
    skos:inScheme <http://opencoredata.org/voc/janus/1/> .

<http://opencoredata.org/voc/janus/1/janusrsc>
    a skos:Concept ;
    skos:definition "Measurements of Reflectance Spectrophotometry and Colorimetry taken on cores using a Minolta CM2002 camera." ;
    skos:inScheme <http://opencoredata.org/voc/janus/1/> .

<http://opencoredata.org/voc/janus/1/janussamplingcode>
    a skos:Concept ;
    skos:definition "NEW:  Codes used to link groups of samples to particular individuals or shipboard laboratories." ;
    skos:inScheme <http://opencoredata.org/voc/janus/1/> .

<http://opencoredata.org/voc/janus/1/janusshearstrengthavs>
    a skos:Concept ;
    skos:definition "Measurements of the torque required to cause a split-core cylindrical surface to be sheared by an automated vane system (AVS)." ;
    skos:inScheme <http://opencoredata.org/voc/janus/1/> .

<http://opencoredata.org/voc/janus/1/janusshearstrengthpen>
    a skos:Concept ;
    skos:definition "Measurements of the unconfined compressive strength of a split-core surface using a pocket penetrometer." ;
    skos:inScheme <http://opencoredata.org/voc/janus/1/> .

<http://opencoredata.org/voc/janus/1/janusshearstrengthtor>
    a skos:Concept ;
    skos:definition "Measurements of shear strength on a split-core using a hand-held Torvane instrument." ;
    skos:inScheme <http://opencoredata.org/voc/janus/1/> .

<http://opencoredata.org/voc/janus/1/janussmearslide>
    a skos:Concept ;
    skos:definition "Quantitative and qualitative abundances at a sample-level of sedimentary components as observed in microscopic smear slides." ;
    skos:inScheme <http://opencoredata.org/voc/janus/1/> .

<http://opencoredata.org/voc/janus/1/janussmearslidecompref>
    a skos:Concept ;
    skos:definition "NEW:  Reference listing of smear slide components." ;
    skos:inScheme <http://opencoredata.org/voc/janus/1/> .

<http://opencoredata.org/voc/janus/1/janusspliceinterval>
    a skos:Concept ;
    skos:definition "NEW:  Summary of core stratigraphic depth correlation between holes at a site derived from downhole depth-shifting and correlation of multiple core and logging datasets." ;
    skos:inScheme <http://opencoredata.org/voc/janus/1/> .

<http://opencoredata.org/voc/janus/1/janussplicetie>
    a skos:Concept ;
    skos:definition "NEW:  Detail of core stratigraphic depth correlation between holes a site derived from downhole depth-shifting and correlation of multiple core and logging datasets." ;
    skos:inScheme <http://opencoredata.org/voc/janus/1/> .

<http://opencoredata.org/voc/janus/1/janussystemsref>
    a skos:Concept ;
    skos:definition "NEW:  Reference for measurement systems" ;
    skos:inScheme <http://opencoredata.org/voc/janus/1/> .

<http://opencoredata.org/voc/janus/1/janustensorcore>
    a skos:Concept ;
    skos:definition "Measurements of magnetic core orientation." ;
    skos:inScheme <http://opencoredata.org/voc/janus/1/> .

<http://opencoredata.org/voc/janus/1/janustensortool>
    a skos:Concept ;
    skos:definition "NEW:  Metadata on Tensor Tool operation." ;
    skos:inScheme <http://opencoredata.org/voc/janus/1/> .

<http://opencoredata.org/voc/janus/1/janusthermalconductivity>
    a skos:Concept ;
    skos:definition "Measurement of thermal conductivity on whole cores after reaching thermal equilibrium in the shipboard laboratory environment using Teka temperature probes." ;
    skos:inScheme <http://opencoredata.org/voc/janus/1/> .

<http://opencoredata.org/voc/janus/1/janusthinsection>
    a skos:Concept ;
    skos:definition "Quantitative and qualitative abundances at a sample-level of sedimentary components as observed in microscopic thin sections." ;
    skos:inScheme <http://opencoredata.org/voc/janus/1/> .

<http://opencoredata.org/voc/janus/1/janusthinsectioncompref>
    a skos:Concept ;
    skos:definition "NEW:  Reference listing of thin section components." ;
    skos:inScheme <http://opencoredata.org/voc/janus/1/> .

<http://opencoredata.org/voc/janus/1/janusthinsectionimage>
    a skos:Concept ;
    skos:definition "URL links to images of thin section microphotographs." ;
    skos:inScheme <http://opencoredata.org/voc/janus/1/> .

<http://opencoredata.org/voc/janus/1/janusvcdhardrockimage>
    a skos:Concept ;
    skos:definition "URL links to scanned images of visual core descriptions (VCD) on hard rocks." ;
    skos:inScheme <http://opencoredata.org/voc/janus/1/> .

<http://opencoredata.org/voc/janus/1/janusvcdimage>
    a skos:Concept ;
    skos:definition "URL links to scanned images of visual core descriptions (VCD)." ;
    skos:inScheme <http://opencoredata.org/voc/janus/1/> .

<http://opencoredata.org/voc/janus/1/janusvcdstructureimage>
    a skos:Concept ;
    skos:definition "URL links to scanned images of visual core descriptions (VCD) on core structure." ;
    skos:inScheme <http://opencoredata.org/voc/janus/1/> .

<http://opencoredata.org/voc/janus/1/janusxrd>
    a skos:Concept ;
    skos:definition "NEW:  Measurements and metadata on X-Ray Diffraction (XRD) samples." ;
    skos:inScheme <http://opencoredata.org/voc/janus/1/> .

<http://opencoredata.org/voc/janus/1/janusxrdimage>
    a skos:Concept ;
    skos:definition "URL links to scanned images of instrumentation output of X-Ray Diffraction (XRD) peak values." ;
    skos:inScheme <http://opencoredata.org/voc/janus/1/> .

<http://opencoredata.org/voc/janus/1/janusxrf>
    a skos:Concept ;
    skos:definition "Measurements of concentrations of major and trace elements from X-Ray Fluorescence (XRF) spectrometry samples." ;
    skos:inScheme <http://opencoredata.org/voc/janus/1/> .

